libcrux-ml-dsa/proofs/fstar/extraction/Libcrux_ml_dsa.Simd.Traits.fst
@@ -3,6 +3,76 @@ module Libcrux_ml_dsa.Simd.Traits
 open Core
 open FStar.Mul
 
-let int_in_i32_range (i: Hax_lib.Int.t_Int) =
+let int_is_i32 (i: Hax_lib.Int.t_Int) =
   i <= (Rust_primitives.Hax.Int.from_machine Core.Num.impl_i32__MAX <: Hax_lib.Int.t_Int) &&
   i >= (Rust_primitives.Hax.Int.from_machine Core.Num.impl_i32__MIN <: Hax_lib.Int.t_Int)
+
+let add_pre (lhs rhs: t_Array i32 (mk_usize 8)) =
+  Hax_lib.v_forall #usize
+    (fun i ->
+        let i:usize = i in
+        Hax_lib.implies (i <. v_COEFFICIENTS_IN_SIMD_UNIT <: bool)
+          (fun temp_0_ ->
+              let _:Prims.unit = temp_0_ in
+              int_is_i32 ((Rust_primitives.Hax.Int.from_machine (lhs.[ i ] <: i32)
+                    <:
+                    Hax_lib.Int.t_Int) +
+                  (Rust_primitives.Hax.Int.from_machine (rhs.[ i ] <: i32) <: Hax_lib.Int.t_Int)
+                  <:
+                  Hax_lib.Int.t_Int)
+              <:
+              bool)
+        <:
+        bool)
+
+let add_post (lhs rhs future_lhs: t_Array i32 (mk_usize 8)) =
+  Hax_lib.v_forall #usize
+    (fun i ->
+        let i:usize = i in
+        Hax_lib.implies (i <. v_COEFFICIENTS_IN_SIMD_UNIT <: bool)
+          (fun temp_0_ ->
+              let _:Prims.unit = temp_0_ in
+              (Rust_primitives.Hax.Int.from_machine (future_lhs.[ i ] <: i32) <: Hax_lib.Int.t_Int) =
+              ((Rust_primitives.Hax.Int.from_machine (lhs.[ i ] <: i32) <: Hax_lib.Int.t_Int) +
+                (Rust_primitives.Hax.Int.from_machine (rhs.[ i ] <: i32) <: Hax_lib.Int.t_Int)
+                <:
+                Hax_lib.Int.t_Int)
+              <:
+              bool)
+        <:
+        bool)
+
+let sub_pre (lhs rhs: t_Array i32 (mk_usize 8)) =
+  Hax_lib.v_forall #usize
+    (fun i ->
+        let i:usize = i in
+        Hax_lib.implies (i <. v_COEFFICIENTS_IN_SIMD_UNIT <: bool)
+          (fun temp_0_ ->
+              let _:Prims.unit = temp_0_ in
+              int_is_i32 ((Rust_primitives.Hax.Int.from_machine (lhs.[ i ] <: i32)
+                    <:
+                    Hax_lib.Int.t_Int) -
+                  (Rust_primitives.Hax.Int.from_machine (rhs.[ i ] <: i32) <: Hax_lib.Int.t_Int)
+                  <:
+                  Hax_lib.Int.t_Int)
+              <:
+              bool)
+        <:
+        bool)
+
+let sub_post (lhs rhs future_lhs: t_Array i32 (mk_usize 8)) =
+  Hax_lib.v_forall #usize
+    (fun i ->
+        let i:usize = i in
+        Hax_lib.implies (i <. v_COEFFICIENTS_IN_SIMD_UNIT <: bool)
+          (fun temp_0_ ->
+              let _:Prims.unit = temp_0_ in
+              (Rust_primitives.Hax.Int.from_machine (future_lhs.[ i ] <: i32) <: Hax_lib.Int.t_Int) =
+              ((Rust_primitives.Hax.Int.from_machine (lhs.[ i ] <: i32) <: Hax_lib.Int.t_Int) -
+                (Rust_primitives.Hax.Int.from_machine (rhs.[ i ] <: i32) <: Hax_lib.Int.t_Int)
+                <:
+                Hax_lib.Int.t_Int)
+              <:
+              bool)
+        <:
+        bool)
